updates

intermediate2/Zeta.Intermediate.Store.fst
@@ -1138,24 +1138,47 @@ let pointing_slot (#vcfg:_)
  assert(madd_props_local st s);
  parent_slot st s
 
-let rec find #vcfg (st: Seq.seq (option (vstore_entry vcfg))) (k: base_key)
-  : Tot (option (Spec.vstore_entry vcfg.app k))
-    (decreases (Seq.length st)) =
-  if Seq.length st = 0 then None
-  else
-    match Seq.head st with
-    | None -> find (Seq.tail st) k
-    | Some (VStoreE (gk,gv) am1 _ _ _) ->
-      let bk1 = to_base_key gk in
-      if bk1 = k then
-        let open Zeta.High.Verifier in
-        let r = gk,gv in
-        let am = am1 in
-        Some ({r; am})
-      else find (Seq.tail st) k
+let store_contains_key_prop (#vcfg:_) (st: vstore vcfg) (k: base_key)
+  = exists (s: slot_id vcfg). (inuse_slot st s /\ stored_base_key st s = k)
 
-let as_map (#vcfg:_) (st:ismap_vstore vcfg) : Spec.store_t vcfg.app
-  = find st
+#push-options "--fuel 0 --ifuel 1 --query_stats"
+
+let rec find_aux (#vcfg:_) (st: vstore vcfg) (k: base_key) (s: nat{ s <= store_size vcfg })
+  : Tot (o:option (slot_id vcfg) {match o with
+                                  | None -> forall s'. (s' < s) ==> (stored_base_key st s' <> k)
+                                  | Some s' -> s' < s /\ inuse_slot st s' /\
+                                               stored_base_key st s' = k})
+    (decreases s)
+  = if s = 0 then None
+    else
+      let s' = s - 1 in
+      if inuse_slot st s' && stored_base_key st s' = k then
+        Some s'
+      else
+        let o = find_aux st k s' in
+        if None = o then (
+          let aux (sx:_)
+            : Lemma (ensures (sx < s ==> stored_base_key st sx <> k))
+            = ()
+          in
+          forall_intro aux;
+          None
+        )
+        else o
+
+#pop-options
+
+let store_contains_key (#vcfg:_) (st:ismap_vstore vcfg) (k:base_key):
+  b:bool{b <==> (exists (s: slot_id vcfg). inuse_slot st s /\ stored_base_key st s = k)}
+  = let o = find_aux st k (store_size vcfg) in
+    Some? o
+
+let slot_of_key
+  (#vcfg:_)
+  (st:ismap_vstore vcfg)
+  (k: base_key{store_contains_key st k})
+  : Tot (s: inuse_slot_id st {k = stored_base_key st s})
+  = Some?.v (find_aux st k (store_size vcfg))
 
 (* updating a value preserves is_map *)
 let lemma_ismap_update_value (#vcfg:verifier_config)
@@ -1180,19 +1203,9 @@ let lemma_ismap_update_value (#vcfg:verifier_config)
     in
     forall_intro_2 aux
 
-let rec seq_contains_key #vcfg (st: Seq.seq (option (vstore_entry vcfg))) (i: seq_index st)
-  : Lemma (requires (Some? (Seq.index st i)))
-          (ensures (let gk,gv = VStoreE?.r (Some?.v (Seq.index st i)) in
-                    let k = to_base_key gk in
-                    Spec.store_contains (find st) k))
-          (decreases (Seq.length st)) =
-  if i = 0 then ()
-  else
-    seq_contains_key (Seq.tail st) (i - 1)
-
 let store_contains_inuse_slot_keys #vcfg (st: ismap_vstore vcfg) (s: inuse_slot_id st)
   : Lemma (ensures (store_contains_key st (stored_base_key st s))) =
-  seq_contains_key st s
+  ()
 
 let lemma_ismap_madd_to_store (#vcfg:_) (st:ismap_vstore vcfg)
   (s:empty_slot_id st)
@@ -1259,12 +1272,6 @@ let lemma_ismap_madd_to_store_split
 
 (* if two slots of an ismap store contain the same key, then the two slots should be identical *)
 let lemma_ismap_correct (#vcfg:_) (st:ismap_vstore vcfg) (s1 s2: inuse_slot_id st)
-  : Lemma (requires (stored_key st s1 = stored_key st s2))
-          (ensures (s1 = s2))
-  = ()
-
-(* if two slots of an ismap store contain the same key, then the two slots should be identical *)
-let lemma_ismap_correct2 (#vcfg:_) (st:ismap_vstore vcfg) (s1 s2: inuse_slot_id st)
   : Lemma (requires (stored_base_key st s1 = stored_base_key st s2))
           (ensures (s1 = s2))
   = ()
@@ -1272,31 +1279,9 @@ let lemma_ismap_correct2 (#vcfg:_) (st:ismap_vstore vcfg) (s1 s2: inuse_slot_id 
 let lemma_empty_store_is_map (#vcfg:_):
   Lemma (ensures (is_map (empty_store vcfg))) = ()
 
-let rec index_of_found #vcfg (st: Seq.seq (option (vstore_entry vcfg))) (k: base_key{Some? (find st k)}):
-  Tot (i: seq_index st{Some? (Seq.index st i) /\
-                       (let gk,gv = VStoreE?.r (Some?.v (Seq.index st i)) in
-                        let bk = to_base_key gk in
-                        bk = k /\
-                        Spec.stored_key (find st) k = gk /\
-                       Spec.stored_value (find st) k = gv /\
-                       Spec.add_method_of (find st) k = VStoreE?.am (Some?.v (Seq.index st i)))})
-  (decreases (Seq.length st)) =
-  match Seq.head st with
-  | None -> 1 + index_of_found (Seq.tail st) k
-  | Some (VStoreE (gk,gv) am1 _ _ _) ->
-    let bk = to_base_key gk in
-    if bk = k then 0
-    else 1 + index_of_found (Seq.tail st) k
-
 let lemma_empty_contains_nokey (#vcfg:_) (k:base_key):
   Lemma (ensures (let st = empty_store vcfg in
-                  not (store_contains_key st k))) =
-  let st = empty_store vcfg in
-  if store_contains_key st k then (
-    let i = index_of_found st k in
-    ()
-  )
-  else ()
+                  not (store_contains_key st k))) = ()
 
 let lemma_madd_root_to_store_is_map
       (#vcfg:_)
@@ -1325,38 +1310,6 @@ let lemma_madd_root_to_store_is_map
         )
     in
     forall_intro_2 aux
-
-let lemma_as_map_empty (vcfg:_)
-  : Lemma (ensures (let st = empty_store vcfg in
-                     forall (k:base_key). as_map st k = None)) =
-  let st = empty_store vcfg in
-  let aux k: Lemma (ensures (as_map st k = None)) [SMTPat (as_map st k)] =
-    lemma_empty_contains_nokey #vcfg k;
-    ()
-  in
-  ()
-
-let lemma_as_map_slot_key_equiv (#vcfg:_) (st:ismap_vstore vcfg) (s:inuse_slot_id _)
-  : Lemma (ensures (let k = stored_base_key st s in
-                    let stk = as_map st in
-                    Spec.store_contains stk k /\
-                    stored_key st s = Spec.stored_key stk k /\
-                    stored_value st s = Spec.stored_value stk k /\
-                    add_method_of st s = Spec.add_method_of stk k)) =
-  store_contains_inuse_slot_keys st s;
-  let k = stored_base_key st s in
-  let stk = as_map st in
-  assert(Spec.store_contains stk k);
-  let s' = index_of_found st k in
-  lemma_ismap_correct2 st s s'
-
-let slot_of_key (#vcfg:_) (st:ismap_vstore vcfg) (k: base_key{let stk = as_map st in
-                                                              Spec.store_contains stk k})
-  : Tot (s: inuse_slot_id st {let stk = as_map st in
-                              k = stored_base_key st s /\
-                              stored_value st s = Spec.stored_value stk k /\
-                              add_method_of st s = Spec.add_method_of stk k})
-  = index_of_found st k
 
 let lemma_not_contains_after_mevict
   (#vcfg: verifier_config)
@@ -1389,7 +1342,7 @@ let lemma_not_contains_after_mevict
     forall_intro_2 aux;
     assert(is_map st_);
     if store_contains_key st_ k then (
-      let s1 = index_of_found st_ k in
+      let s1 = slot_of_key st_ k in
       assert(s1 <> s);
       assert(stored_base_key st s1 = k);
       ()
@@ -1423,78 +1376,11 @@ let lemma_not_contains_after_bevict
     forall_intro_2 aux;
     assert(is_map st_);
     if store_contains_key st_ k then (
-      let s1 = index_of_found st_ k in
+      let s1 = slot_of_key st_ k in
       assert(s1 <> s);
       assert(stored_base_key st s1 = k);
       ()
     )
-
-let madd_to_store_root_as_map_aux (#vcfg:_) (st:vstore vcfg) (s:empty_slot_id st)
-  (v:value vcfg.app{IntV? v})
-  : Lemma (requires (is_map st /\ ~ (store_contains_key st Root)))
-          (ensures (is_map (madd_to_store_root st s v) /\
-                    FE.feq (as_map (madd_to_store_root st s v))
-                           (Spec.add_to_store (as_map st) (IntK Root, v) Spec.MAdd)))
-  = let st1 = madd_to_store_root st s v in
-    lemma_madd_root_to_store_is_map st s v;
-    assert(is_map st1);
-    let stk = as_map st in
-    let stk1 = Spec.add_to_store stk (IntK Root, v) Spec.MAdd in
-    let stk1' = as_map st1 in
-    let aux (k:_):
-      Lemma (ensures (stk1' k = stk1 k))
-      [SMTPat (stk1' k); SMTPat (stk1 k)] =
-      if k = Root then ()
-      else if Spec.store_contains stk1' k then (
-        assert(store_contains_key st1 k);
-        let sk = slot_of_key st1 k in
-        assert(sk <> s);
-        assert(stored_base_key st sk = k);
-        lemma_as_map_slot_key_equiv st1 sk;
-
-        assert(stored_key st1 sk = Spec.stored_key stk1' k);
-        assert(stored_value st1 sk = Spec.stored_value stk1' k);
-        assert(add_method_of st1 sk = Spec.add_method_of stk1' k);
-
-        assert(stored_key st1 sk = stored_key st sk);
-        assert(stored_value st1 sk = stored_value st sk);
-        assert(add_method_of st1 sk = add_method_of st sk);
-
-        lemma_as_map_slot_key_equiv #vcfg st sk;
-        (* TODO: this is the expansion of lemma ensures above - why is it failing? *)
-        assume(let s = sk in
-               let k = stored_base_key st s in
-               let stk = as_map st in
-               Spec.store_contains stk k /\
-               stored_key st s = Spec.stored_key stk k /\
-               stored_value st s = Spec.stored_value stk k /\
-               add_method_of st s = Spec.add_method_of stk k);
-        ()
-      )
-      else if Spec.store_contains stk1 k then (
-        assert(Spec.store_contains stk k);
-        let sk = slot_of_key st k in
-        assert(stored_base_key st1 sk = k);
-        admit()
-      )
-      else
-        ()
-    in
-    ()
-
-
-let madd_to_store_root_as_map (#vcfg:_) (st:vstore vcfg) (s:empty_slot_id st)
-  (v:value vcfg.app{IntV? v})
-  : Lemma (is_map st /\ ~ (store_contains_key st Root) ==>
-                  is_map (madd_to_store_root st s v) /\
-                  FE.feq (as_map (madd_to_store_root st s v))
-                         (Spec.add_to_store (as_map st) (IntK Root, v) Spec.MAdd))
-  = introduce
-    is_map st /\ ~ (store_contains_key st Root) ==>
-                  is_map (madd_to_store_root st s v) /\
-                  FE.feq (as_map (madd_to_store_root st s v))
-                         (Spec.add_to_store (as_map st) (IntK Root, v) Spec.MAdd)
-    with _. (madd_to_store_root_as_map_aux st s v)
 
 let lemma_ismap_badd_to_store (#vcfg:_) (st:ismap_vstore vcfg)
   (s:empty_slot_id st)
@@ -1524,11 +1410,16 @@ let lemma_ismap_badd_to_store (#vcfg:_) (st:ismap_vstore vcfg)
     forall_intro_2 aux;
     ()
 
+#push-options "--fuel 0 --ifuel 1 --query_stats"
+
 let store_rel_slot (#vcfg:_) (st: ismap_vstore vcfg) (st':_ {store_rel st st'}) (s: inuse_slot_id st)
   : Lemma (ensures (let k = stored_base_key st s in
                     Spec.store_contains st' k /\
                     stored_key st s = Spec.stored_key st' k /\
                     stored_value st s = Spec.stored_value st' k /\
                     add_method_of st s = Spec.add_method_of st' k))
-  = lemma_as_map_slot_key_equiv st s;
-    admit()
+  = let k = stored_base_key st s in
+    store_contains_inuse_slot_keys st s;
+    lemma_ismap_correct st s (slot_of_key st k)
+
+#pop-options
